heap_model.v
@@ -96,24 +96,22 @@ Fixpoint extractSome (f : adr -> option adr) (li : list adr) : list adr :=
                  end
   end.
 
-Lemma world_finite: forall w: world, exists l: list adr, forall a:adr, (In a l -> lookup_fpm w a <> None) /\
-                                                                       (~ In a l -> lookup_fpm w a = None).
+Lemma world_finite: forall w: world, exists l: list adr, forall a:adr, In a l <-> lookup_fpm w a <> None.
 Proof.
-  intro. destruct w as [f [li H]]. simpl. exists (extractSome f li).
-  split; intros.
-  clear H.
-  induction li; simpl in H0. auto.
-  destruct (f a0) eqn: ?.
-  destruct (in_inv H0). rewrite <- H, Heqo. intro HH; inversion HH.
-  apply IHli; auto. apply IHli; auto.
-  destruct (in_dec nat_eq_dec a li).
-  clear H. induction li. simpl in *; exfalso; auto.
-  simpl in H0. destruct (f a0) eqn : ?.
-  apply IHli.
-  intro; apply H0. apply in_cons; auto.
-  destruct (in_inv i). rewrite H in H0. exfalso; apply H0, in_eq. auto.
-  destruct (in_inv i). rewrite H in Heqo; auto. apply IHli; auto.
-  apply H; auto.
+  intro; destruct w as [f [li ?]]; simpl; exists (extractSome f li); split; intros.
+  clear e; induction li; simpl in H; auto.
+  destruct (f a0) eqn: ?. destruct (in_inv H). subst. rewrite Heqo. intro. inversion H0.
+  apply IHli; auto. apply IHli; auto. destruct (in_dec nat_eq_dec a li). clear e.
+  induction li; simpl in *; auto. destruct (f a0) eqn : ?. destruct i. subst. apply in_eq.
+  apply in_cons. apply IHli; auto. destruct i. subst. exfalso; auto. apply IHli; auto.
+  specialize (e a n). exfalso; auto.
+Qed.
+
+Lemma lookup_fpm_join_sub: forall (w1 w2 : world) x, join_sub w1 w2 -> lookup_fpm w1 x <> None -> lookup_fpm w2 x <> None.
+Proof.
+  intros. destruct H as [w3 ?].
+  destruct w1 as [f1 [l1 ?]]. destruct w2 as [f2 [l2 ?]]. destruct w3 as [f3 [l3 ?]]. hnf in H; simpl in *.
+  specialize (H x). inversion H. exfalso; auto. auto. auto.
 Qed.
 
 (* Definition equal (x y: var) : pred world := fun w => fst w x = fst w y. *)
